Define i_bind_post without match

iodiv/TestTauIODiv.fst
@@ -16,13 +16,11 @@ open DivFree
 open DivFreeTauSpec
 open DivFreeTauDM
 
-// assume val get_trace : unit -> IODiv trace (fun hist -> True) (ensures fun hist r -> terminates r /\ result r == hist)
-
 let test_1 (s : string) : IODiv string (requires fun h -> True) (ensures fun _ _ -> True) =
   let fd = open_file s in
   read fd
 
-let test_1' (s : string) : IODiv string (requires fun _ -> True) (ensures fun _ _ -> True) 
+let test_1' (s : string) : IODiv string (requires fun _ -> True) (ensures fun _ _ -> True)
 = let fd = open_file s in
   let fd' = open_file s in
   read fd
@@ -36,25 +34,28 @@ let test (s : string) : IODiv unit (requires fun _ -> True) (ensures fun _ _ -> 
   let msg = read fd in
   close fd
 
-let test_ (s : string) : IODiv unit (requires fun _ -> True) (ensures fun hist r -> terminates r /\ (exists fd msg. ret_trace r == [ EOpenFile s fd ; ERead fd msg ; EClose fd ])) by (
+let test_ (s : string) : IODiv unit (requires fun _ -> True) (ensures fun hist r -> terminates r /\ (exists fd msg. ret_trace r == [ EOpenFile s fd ; ERead fd msg ; EClose fd ]))
+by (
   explode ();
-  bump_nth 4; 
-  branch_on_match ();
-  explode ();
-  bump_nth 2;
-  branch_on_match ();
-  explode ();
-  bump_nth 2;
-  norm [delta_only [`%ishift_post; `%ishift_post']; iota];
-  branch_on_match ();
-  let r = instantiate (nth_binder 3) (fresh_uvar None) in
-  mapply r; clear r;
-  explode ();
-  bump_nth 2;
-  let fd = nth_binder 7 in
-  let msg = nth_binder 13 in
-  witness (fd); witness (msg);
-  tadmit (); (** this looks like something that can be solved using a pattern/lemma **)
+  bump_nth 6 ;
+  compute () ;
+  // bump_nth 4;
+  // branch_on_match ();
+  // explode ();
+  // bump_nth 2;
+  // branch_on_match ();
+  // explode ();
+  // bump_nth 2;
+  // norm [delta_only [`%ishift_post; `%ishift_post']; iota];
+  // branch_on_match ();
+  // let r = instantiate (nth_binder 3) (fresh_uvar None) in
+  // mapply r; clear r;
+  // explode ();
+  // bump_nth 2;
+  // let fd = nth_binder 7 in
+  // let msg = nth_binder 13 in
+  // witness (fd); witness (msg);
+  // tadmit (); (** this looks like something that can be solved using a pattern/lemma **)
   dump "H")
 = let fd = open_file s in
   let msg = read fd in
@@ -147,8 +148,8 @@ let pure_lemma_test () : IODiv unit (requires fun _ -> True) (ensures fun _ _ ->
   pure_lemma () ;
   some_f ()
 
-let pure_lemma_test2 () : IODiv unit (requires fun _ -> True) (ensures fun _ _ -> True) by 
- (explode (); bump_nth 9; 
+let pure_lemma_test2 () : IODiv unit (requires fun _ -> True) (ensures fun _ _ -> True) by
+ (explode (); bump_nth 9;
    (** why is this ishift_post needed since it is unfolded by post-processing in
        i_bind? **)
    norm [delta_only [`%ishift_post;`%ishift_post']];
